working on environment projections and finite set of participants

theories/Global.v
@@ -524,6 +524,45 @@ Section Semantics.
            (CONT : lbl /-> mty * ig_ty).
   Set Elimination Schemes.
 
+
+  Inductive part_of: role -> rg_ty -> Prop :=
+    | pof_from F T C: part_of F (rg_msg F T C)
+    | pof_to F T C: part_of T (rg_msg F T C)
+    | pof_cont p F T C L G Ty: C L = Some (Ty, G) 
+      -> part_of p G -> part_of p (rg_msg F T C).
+
+
+
+  Inductive iPart_of: role -> ig_ty -> Prop :=
+    | ipof_end p cG: part_of p cG -> iPart_of p (ig_end cG)
+    | ipof_from o F T C: iPart_of F (ig_msg o F T C)
+    | ipof_to o F T C: iPart_of T (ig_msg o F T C)
+    | ipof_cont p o F T C L G Ty: C L = Some (Ty, G) 
+      -> iPart_of p G -> iPart_of p (ig_msg o F T C).
+
+  Lemma iPart_of_label_label_aux p o o' F T C GG: 
+    iPart_of p GG -> GG = ig_msg o F T C ->
+        iPart_of p (ig_msg o' F T C).
+  Proof.
+  elim.
+  + by [].
+  + by move=> o0 F0 T0 C0 [hp1 hp2 hp3 hp4]; rewrite hp2; apply ipof_from.
+  + by move=> o0 F0 T0 C0 [hp1 hp2 hp3 hp4]; rewrite hp3; apply ipof_to.
+  + move=> p0 o0 F0 T0 C0 L G Ty contL ipartof ih [eq1 eq2 eq3 eq4].
+    by rewrite -eq4; apply: (ipof_cont o' F T contL ipartof).
+  Qed.
+
+  Lemma iPart_of_label_label p o o' F T C: 
+    iPart_of p (ig_msg o F T C) ->
+        iPart_of p (ig_msg o' F T C).
+  Proof.
+  by move=> hp; apply: (@iPart_of_label_label_aux p o o' F T C _ hp).
+  Qed.
+
+
+
+
+
   Definition P_option A (P : A -> Prop) (C : option A) : Prop :=
     match C with
     | Some X => P X
